Add proofs for portable compress module

libcrux-ml-kem/proofs/fstar/extraction/Libcrux_ml_kem.Vector.Portable.Compress.fsti
@@ -41,12 +41,12 @@ val compress_message_coefficient (fe: u16)
         fun result ->
           let result:u8 = result in
           Hax_lib.implies ((Rust_primitives.mk_u16 833 <=. fe <: bool) &&
-              (fe <=. Rust_primitives.mk_u16 2596 <: bool))
+              (fe <=. Rust_primitives.mk_u16 2496 <: bool))
             (fun temp_0_ ->
                 let _:Prims.unit = temp_0_ in
                 result =. Rust_primitives.mk_u8 1 <: bool) &&
           Hax_lib.implies (~.((Rust_primitives.mk_u16 833 <=. fe <: bool) &&
-                (fe <=. Rust_primitives.mk_u16 2596 <: bool))
+                (fe <=. Rust_primitives.mk_u16 2496 <: bool))
               <:
               bool)
             (fun temp_0_ ->
@@ -84,7 +84,18 @@ val compress_1_ (a: Libcrux_ml_kem.Vector.Portable.Vector_type.t_PortableVector)
 
 val decompress_ciphertext_coefficient
       (v_COEFFICIENT_BITS: i32)
-      (v: Libcrux_ml_kem.Vector.Portable.Vector_type.t_PortableVector)
+      (a: Libcrux_ml_kem.Vector.Portable.Vector_type.t_PortableVector)
     : Prims.Pure Libcrux_ml_kem.Vector.Portable.Vector_type.t_PortableVector
-      Prims.l_True
-      (fun _ -> Prims.l_True)
+      (requires
+        (v v_COEFFICIENT_BITS == 4 \/ v v_COEFFICIENT_BITS == 5 \/ v v_COEFFICIENT_BITS == 10 \/
+          v v_COEFFICIENT_BITS == 11) /\
+        (forall (i: nat).
+            i < 16 ==>
+            v (Seq.index a.f_elements i) >= 0 /\
+            v (Seq.index a.f_elements i) < pow2 (v v_COEFFICIENT_BITS)))
+      (ensures
+        fun result ->
+          let result:Libcrux_ml_kem.Vector.Portable.Vector_type.t_PortableVector = result in
+          forall (i: nat).
+            i < 16 ==>
+            v (Seq.index result.f_elements i) < Libcrux_ml_kem.Vector.Traits.v_FIELD_MODULUS)
